

Question:

$$\text{Evaluate : } \int_0^\infty \frac{\sin(x) \sin(2x) \sin(3x)}{x^3} dx.$$

Rewrite as:

$$\text{Evaluate } \int_0^\infty \frac{(\sin x \sin 2x \sin 3x) dx}{x^3}.$$

First, apply the trigonometric identity for the product of three sine functions:

$$\sin a \sin b \sin c = \frac{1}{4} [\sin(a + b - c) + \sin(b + c - a) + \sin(c + a - b) - \sin(a + b + c)].$$

Substituting $a = x$, $b = 2x$, $c = 3x$:

$$\sin x \sin 2x \sin 3x = \frac{1}{4} [\sin(0 \cdot x) + \sin(4x) + \sin(2x) - \sin(6x)] = \frac{1}{4} (\sin 2x + \sin 4x - \sin 6x).$$

Thus, the integral becomes:

$$\int_0^\infty \frac{(\sin x \sin 2x \sin 3x) dx}{x^3} = \frac{1}{4} \int_0^\infty \frac{(\sin 2x + \sin 4x - \sin 6x) dx}{x^3}.$$

Express $1/x^3$ using its integral representation derived from Gamma function:

$$\frac{1}{x^3} = \frac{1}{2} \int_0^\infty t^2 e^{-tx} dt, \quad x > 0.$$

Substitute this into the integral:

$$\frac{1}{4} \int_0^\infty \left(\frac{1}{2} \int_0^\infty t^2 e^{-tx} dt \right) (\sin 2x + \sin 4x - \sin 6x) dx.$$

Interchange the order of integration

(justified by Fubini's theorem given convergence):

$$\frac{1}{8} \int_0^\infty t^2 \left[\int_0^\infty e^{-tx} (\sin 2x + \sin 4x - \sin 6x) dx \right] dt.$$

The inner integral is the Laplace transform:

$$\mathcal{L}\{\sin mx\}(t) = \frac{m}{t^2 + m^2}.$$

Thus:

$$\int_0^\infty e^{-tx} \sin 2x dx = \frac{2}{t^2 + 4}, \quad \int_0^\infty e^{-tx} \sin 4x dx = \frac{4}{t^2 + 16}, \quad \int_0^\infty e^{-tx} \sin 6x dx = \frac{6}{t^2 + 36}.$$

The expression simplifies to:

$$\frac{1}{8} \int_0^\infty t^2 \left(\frac{2}{t^2 + 4} + \frac{4}{t^2 + 16} - \frac{6}{t^2 + 36} \right) dt.$$

Rewrite each term:

$$\frac{t^2}{t^2 + b} = 1 - \frac{b}{t^2 + b}.$$

So:

$$\begin{aligned} 2 \left(1 - \frac{4}{t^2 + 4} \right) + 4 \left(1 - \frac{16}{t^2 + 16} \right) - 6 \left(1 - \frac{36}{t^2 + 36} \right) &= 2 + 4 - 6 - \frac{8}{t^2 + 4} - \frac{64}{t^2 + 16} + \frac{216}{t^2 + 36} \\ &= -\frac{8}{t^2 + 4} - \frac{64}{t^2 + 16} + \frac{216}{t^2 + 36}. \end{aligned}$$

Now integrate:

$$\int_0^\infty \frac{1}{t^2 + a^2} dt = \frac{\pi}{2a}.$$

Thus:

$$\int_0^\infty \left(-\frac{8}{t^2 + 4} - \frac{64}{t^2 + 16} + \frac{216}{t^2 + 36} \right) dt = -8 \cdot \frac{\pi}{4} - 64 \cdot \frac{\pi}{8} + 216 \cdot \frac{\pi}{12} = -2\pi - 8\pi + 18\pi = 8\pi.$$

Finally:

$$\frac{1}{8} \cdot 8\pi = \pi.$$